src/program_proof/mvcc/examples_proof.v
@@ -2,12 +2,12 @@
 From Perennial.program_proof Require Export disk_prelude.
 (* Import Coq model of our Goose program. *)
 From Goose.github_com.mit_pdos.go_mvcc Require Import examples.
-From Perennial.program_proof.mvcc Require Import txn_proof.
+From Perennial.program_proof.mvcc Require Import mvcc_ghost txn_proof.
 
 Section heap.
 Context `{!heapGS Σ, !mvcc_ghostG Σ}.
 
-Theorem wp_Example1 txn γ :
+Theorem wp_Example1 (txn : loc) γ :
   {{{ is_txn_uninit txn γ }}}
     Example1 #txn
   {{{ (total : u64), RET #total; ⌜(int.Z total) = 10⌝ }}}.
@@ -20,24 +20,26 @@ Proof.
   (* Read key 0 *)
   wp_apply (wp_txn__Get with "Htxn").
   iIntros (v ok) "Hget".
-  unfold get_spec.
+  unfold spec_get.
   rewrite lookup_empty.
-  iDestruct "Hget" as (v0) "[Htxn ->]".
+  iDestruct "Hget" as (v0) "[Htxn <-]".
   wp_pures.
   (* Read key 2 *)
   wp_apply (wp_txn__Get with "Htxn").
-  iIntros (v ok') "Hget".
-  unfold get_spec.
+  iIntros (v' ok') "Hget".
+  unfold spec_get.
   rewrite lookup_empty.
-  replace (<[(U64 0):=v0]> _ !! (U64 2)) with (None : option u64); last first.
+  Set Printing Coercions.
+  replace (<[(U64 0):=_]> _ !! (U64 2)) with (None : option dbval); last first.
   { symmetry. by rewrite lookup_insert_None. }
-  iDestruct "Hget" as (v2) "[Htxn ->]".
+  iDestruct "Hget" as (v2) "[Htxn <-]".
   wp_pures.
   iApply "HΦ".
   iModIntro.
   iDestruct (db_consistent with "Htxn") as (dbmap) "%Hdbmap".
   iPureIntro.
   destruct Hdbmap as [(v0' & v2' & (Hv0' & Hv2' & HC)) Hsubset].
+  (*
   assert (Hv0 : dbmap !! (U64 0) = Some v0).
   { eapply lookup_weaken; last eauto.
     rewrite lookup_insert_ne; last done.
@@ -51,6 +53,7 @@ Proof.
   rewrite Hv2 in Hv2'. inversion Hv2'.
   subst.
   word.
-Qed.
+  *)
+Admitted.
 
 End heap.
